Petrinets done

petrinet.v
@@ -3,27 +3,47 @@ From iris.algebra Require Import auth frac agree gmap.
 From iris_io Require Export lang rules.
 From iris.proofmode Require Import tactics.
 
+Require Import Coq.Logic.FunctionalExtensionality.
+
 Section PetriNet.
 
-  Context `{EqDecision Pl}.
+  Class PlacesC := places
+      { Places : Type;
+        ThePlaces_eqdec :> EqDecision Places;
+      }.
+
+  Context `{PlacesC}.
 
   Inductive Transition : Type :=
-    IOTr (p : Pl) (t : ioTag) (v v' : val) (q : Pl)
-  | SplitTr (p q q': Pl)
-  | JoinTr (p p' q: Pl)
-  | NoOpTr (p q : Pl).
+    IOTr (p : Places) (t : ioTag) (v v' : val) (q : Places)
+  | SplitTr (p q q': Places)
+  | JoinTr (p p' q: Places)
+  | NoOpTr (p q : Places).
 
   Definition PetriNet := Transition → Prop.
 
-  Definition Valuation := Pl → nat.
+  (** The CMRA for petrinet valuations. *)
+  Class petrinetIG Σ := PetriNetIG {
+    γPN : gname;
+    PNI_exclG :> inG Σ (authUR (ofe_funUR (λ p : Places, natUR)));
+    ThePetriNet : PetriNet
+  }.
 
   Implicit Types N : PetriNet.
+  Implicit Types p q : Places.
+
+  Definition Valuation := Places → nat.
+
   Implicit Types V : Valuation.
-  Implicit Types p q : Pl.
 
   Definition singVAL p := (λ q, if decide (p = q) then 1 else 0).
 
   Definition ValPlus V V' := λ p, V p + V' p.
+
+  Global Instance : Comm eq ValPlus.
+  Proof.
+    intros x y. extensionality u; unfold ValPlus; omega.
+  Qed.
 
   Notation "V ⊎ W" := (ValPlus V W) (at level 50, left associativity).
 
@@ -46,18 +66,12 @@ Section PetriNet.
       Traces N (singVAL q ⊎ V) τ →
       Traces N (singVAL p ⊎ V) τ.
 
-  Definition ResultDet N V :=
-    ∀ t v v' v'' τ,
-      Traces N V (τ ++ [(t, v, v')]) →
-      Traces N V (τ ++ [(t, v, v'')]) → v' = v''.
+  Definition ResultDet (T : ioSpec) :=
+    ∀ t v v' v'' τ τ' τ'',
+      T (τ ++ (t, v, v') :: τ') →
+      T (τ ++ (t, v, v'') :: τ'') → v' = v''.
 
-  (** The CMRA for petrinet valuations. *)
-  Class petrinetIG Σ := PetriNetIG {
-    PNI_exclG :> inG Σ (authUR (ofe_funUR (λ p : Pl, natUR)));
-    γPN : gname
-  }.
-
-  Context `{petrinetIG Σ}.
+  Context `{heapIG Σ, petrinetIG Σ}.
 
   Program Definition FullVAL V :=
     @own Σ (authUR (ofe_funUR (λ p, natUR))) _ γPN (● V).
@@ -65,16 +79,141 @@ Section PetriNet.
   Definition ownVAL V :=
     @own Σ (authUR (ofe_funUR (λ p, natUR))) _ γPN (◯ V).
 
-  Definition Token p := ownVAL (singVAL p).
-
-  Lemma OwnVAL_split V V' : ownVAL (V ⊎ V') ⊣⊢ ownVAL V ∗  ownVAL V'.
+  Lemma ownVAL_split V V' : ownVAL (V ⊎ V') ⊣⊢ ownVAL V ∗  ownVAL V'.
   Proof. by rewrite /ownVAL -own_op -auth_frag_op. Qed.
 
-  Context {N}.
+  Global Instance of_fun_CmraDiscrete (A : Type) (f : A → ucmraT) :
+    (∀ x, CmraDiscrete (f x)) → CmraDiscrete (ofe_funUR f).
+  Proof.
+    intros Hfx; split.
+    - intros z z' Heq u.
+      destruct (Hfx u) as [Hfxo _].
+      apply Hfxo; apply Heq.
+    - intros x Hx0 u.
+      destruct (Hfx u) as [_ Hfxv].
+      apply Hfxv.
+      apply Hx0.
+  Qed.
 
-  
+  Lemma ownVAL_Full V V' : ownVAL V -∗ FullVAL V' -∗ ⌜∃ V'', V' = V ⊎ V''⌝.
+  Proof.
+    iIntros "H1 H2".
+    iCombine "H1" "H2" as "H".
+    iDestruct (own_valid with "H") as "Hvl".
+    iDestruct "Hvl" as %Hvl.
+    rewrite auth_valid_eq in Hvl; simpl in *; destruct Hvl as [Hvl _].
+    specialize (Hvl 0).
+    apply cmra_discrete_included_iff in Hvl.
+    revert Hvl; rewrite right_id; intros [V'' Hvl].
+    iPureIntro.
+    exists V''. extensionality p.
+    apply Hvl.
+  Qed.
+
+  Definition PetriNetN := (nroot .@ "PetriNet").
+
+  Definition PetriNetInv : iProp Σ :=
+    inv PetriNetN (∃ V T, ownIO T ∗ FullVAL V ∗
+                                ⌜∀ τ, Traces ThePetriNet V τ → T τ⌝ ∗ ⌜ResultDet T⌝)%I.
+
+  Definition Token p := (ownVAL (singVAL p) ∗ PetriNetInv)%I.
+
+  Lemma PetriNet_delete V V' : FullVAL (V ⊎ V') -∗ ownVAL V' -∗ |==> FullVAL V.
+  Proof.
+    iIntros "Hf Ho".
+    rewrite /FullVAL /ownVAL.
+    iCombine "Hf" "Ho" as "Hfo".
+    iMod (own_update with "Hfo") as "Hf".
+    { apply auth_update_dealloc.
+      apply (local_update_unital_discrete _ _ (V : (ofe_funUR (λ p, natUR)))).
+      intros z Hvl Heq; split ; first done.
+      rewrite left_id; intros u.
+      specialize (Heq u); simpl in *.
+      apply leibniz_equiv in Heq.
+      assert (V u + V' u = V' u + z u) as Heq' by apply Heq.
+      assert (V u = z u) by omega.
+      done. }
+    done.
+  Qed.
+
+  Lemma PetriNet_alloc V V' : FullVAL V -∗ |==> FullVAL (V ⊎ V') ∗ ownVAL V'.
+  Proof.
+    iIntros "Hf".
+    iMod (own_update with "Hf") as "Hfo".
+    { apply auth_update_alloc.
+      apply (local_update_unital_discrete
+               _ _ (V ⊎ V' : (ofe_funUR (λ p, natUR))) V').
+      intros z Hvl Heq; split ; first done.
+      revert Heq; rewrite left_id => Heq.
+      by intros u; rewrite (comm _ _ z) /ValPlus; rewrite (Heq u). }
+    iDestruct "Hfo" as "[Hf Ho]".
+    by iFrame.
+  Qed.
+
+  Lemma wp_petrinet_io t e v p v' q :
+    IntoVal e v →
+    ThePetriNet (IOTr p t v v' q) →
+    {{{Token p}}} IO t e {{{RET v'; Token q}}}.
+  Proof.
+    iIntros (<-%of_to_val HIO Φ) "[Htk #Hinv] HΦ".
+    iApply wp_atomic.
+    iInv PetriNetN as "Hpt" "Hcl".
+    iDestruct "Hpt" as (V T) "(HT & HV & >Hinc & >Hrd)".
+    iDestruct "Hinc" as %Hinc. iDestruct "Hrd" as %Hrd.
+    iModIntro.
+    iMod "HV".
+    iDestruct (ownVAL_Full with "Htk HV") as (V'') "#HV''".
+    iDestruct "HV''" as %HV''; subst.
+    iApply (wp_io with "[$HT]"); eauto.
+    { apply Hinc. repeat econstructor; eauto. }
+    iNext. iIntros (w) "[HT HTw]". iDestruct "HTw" as %HTw.
+    rewrite (comm _ _ V'').
+    iMod (PetriNet_delete with "HV Htk") as "HV".
+    iMod (PetriNet_alloc _ (singVAL q) with "HV") as "[HV Htk]".
+    assert (w = v'); subst.
+    { eapply (Hrd _ _ _ _ [] [] []).
+      - by apply HTw.
+      - apply Hinc. repeat econstructor; eauto. }
+    iMod ("Hcl" with "[HT HV]") as "_".
+    iNext; iExists _, _; iFrame; iSplit; iPureIntro.
+    - intros τ Hτ.
+      apply Hinc.
+      econstructor; eauto.
+      by rewrite (comm _ _ V'').
+    - intros t' u u' u'' τ τ' τ'' HT1 HT2.
+      eapply (Hrd _ _ _ _ (_ :: _)); eauto.
+    - iModIntro. by iApply ("HΦ" with "[$Htk]").
+  Qed.
 
 End PetriNet.
 
-Notation "V ⊎ W" := (ValPlus V W) (at level 50, left associativity).
+Arguments PetriNet _, {_}.
 
+Section PetriNetInv.
+
+  Context `{heapIG Σ, PlacesC}.
+
+  Lemma PetriNetInv_alloc (N : PetriNet) E (V : (ofe_funUR (λ p, natUR))) :
+    inG Σ (authUR (ofe_funUR (λ p : Places, natUR))) →
+    ResultDet (Traces N V) →
+    ownIO (Traces N V) ⊢
+          |={E}=> ∃ `{PIG : !petrinetIG Σ}, PetriNetInv ∗ ownVAL V.
+  Proof.
+    iIntros (Hing Hrd) "HIO".
+    iMod (@own_alloc Σ (authUR (ofe_funUR (λ p, natUR))) _ ((◯ V) ⋅ (● V)))
+      as (γpn) "[Hofrag Hofull]".
+    { rewrite auth_valid_eq; simpl; split; last done.
+        by intros; rewrite right_id. }
+    set (HIG := {| PNI_exclG := Hing; γPN := γpn; ThePetriNet := N|}).
+    iMod (inv_alloc
+            PetriNetN _
+            (∃ V T, ownIO T ∗ FullVAL V ∗
+                          ⌜∀ τ, Traces N V τ → T τ⌝ ∗ ⌜ResultDet T⌝)%I
+            with "[Hofull HIO]") as "Hinv".
+    { iNext; iExists _, _; iFrame; iSplit; iPureIntro; auto. }
+    iModIntro; iExists _; iFrame.
+  Qed.
+
+End PetriNetInv.
+
+Notation "V ⊎ W" := (ValPlus V W) (at level 50, left associativity).
